Implementation almost done; need to do asSeq() method

proj/TreeSet.dfy
@@ -1,133 +1,495 @@
-// Function type for comparing elements
-// TODO: depois ver se consigo por tipo generico mesmo
 type T = int // for demo purposes, but could be real, etc.
+
+// TODO: ver melhor as clauses/ensures e isso com o Repr
+
+// helper function to check if a value is the smallest element in a set
+predicate isMin(x: T, arr: set<T>)
+{
+  forall elem :: elem in arr ==> x <= elem
+}
+
+// helper function to check if a sequence is in strictly increasing order
+predicate isSorted(arr: seq<T>)
+{
+  forall k1, k2 :: 0 <= k1 < k2 < |arr| ==> arr[k1] < arr[k2]
+}
 
 // **********************************************************************
 // Represents a binary search tree node, for elements of type T.
+class {:autocontracts} BSTNode {
+  // ghost variable representing a set of all the elems that are in the BST which root is this node
+  ghost var elems: set<T>;
 
-class BTNode {
-  var value: T; // value of the node
-  var left: BTNode?;  // left child of the node (? - may be null)
-  var right: BTNode?; // right child of the node (? - may be null)
+  // ghost variable representing a set of all the node objects that are in the BST which root is this node
+  ghost var Repr: set<object>;
 
-  // Constructor of the class.
-  constructor (value: T, left: BTNode?, right: BTNode?) 
-    ensures this.value == value
-    ensures this.left == left
-    ensures this.right == right
+  // value of the node
+  var value: T;
+
+  // left child of the node (? - may be null)
+  var left: BSTNode?;
+
+  // right child of the node (? - may be null)
+  var right: BSTNode?;
+
+  // class invariant of the BSTNode class
+  predicate Valid()
   {
-    this.value := value;
-    this.left := left;
-    this.right := right;
+    // check if this node is in Repr
+    this in Repr &&
+
+    // check correctness for left subtree:
+    // check if Repr contains left and all nodes of the left subtree
+    // check if left's Repr does not contain the current node, to avoid cycles
+    // check class invariant for left node
+    // check if all nodes on left subtree are less than the current node
+    (left != null ==> 
+      left in Repr &&
+      left.Repr <= Repr && this !in left.Repr &&
+      left.Valid() &&
+      (forall elem :: elem in left.elems ==> elem < value)) &&
+
+    // check correctness for right subtree:
+    // check if Repr contains right and all nodes of the right subtree
+    // check if right's Repr does not contain the current node, to avoid cycles
+    // check class invariant for right node
+    // check if all nodes on right subtree are higher than the current node
+    (right != null ==> 
+      right in Repr &&
+      right.Repr <= Repr && this !in right.Repr &&
+      right.Valid() &&
+      (forall elem :: elem in right.elems ==> value < elem)) &&
+
+    // case where the node does not have any subtrees:
+    // connect ghost variable elems with its intended value
+    (left == null && right == null ==>
+      elems == {value}) &&
+
+    // case where only left subtree exists:
+    // connect ghost variable elems with its intended value
+    (left != null && right == null ==>
+      elems == left.elems + {value}) &&
+
+    // case where only right subtree exists:
+    // connect ghost variable elems with its intended value
+    (left == null && right != null ==>
+      elems == {value} + right.elems) &&
+
+    // case where both left and right subtrees exist:
+    // check if left and right subtrees are disjoint (i.e. no node belongs to both)
+    // connect ghost variable elems with its intended value
+    (left != null && right != null ==>
+      left.Repr !! right.Repr &&
+      elems == left.elems + {value} + right.elems)
+  }
+
+  // constructor of the class. Creates a single node with no children
+  constructor (data: T) 
+    ensures elems == {data}
+    ensures Repr == {this}
+  {
+    value := data;
+    left := null;
+    right := null;
+    elems := {data};
+    Repr := {this};
+  }
+
+  // method that checks if a given value is present in the BST
+  function method contains(x: T) : bool
+    ensures contains(x) <==> x in elems
+  {
+    // if value is equal to the root, return true
+    if x == value then true
+    
+    // if the value is smaller, check on left subtree 
+    else if left != null && x < value then left.contains(x)
+
+    // if the value is higher, check on right subtree
+    else if right != null && x > value then right.contains(x)
+
+    // value is not present in the BST
+    else false
+  }
+
+  // method that deletes a value from the BST
+  // returns the new root of the tree (null if the last node of the BST has been deleted)
+  method delete(x: T) returns (node: BSTNode?)
+    decreases Repr
+    ensures fresh(Repr - old(Repr))
+    ensures node == null ==> old(elems) <= {x}
+    ensures node != null ==> node.Valid() && node.Repr <= Repr && node.elems == old(elems) - {x}
+  {
+    node := this;
+    // if the 'x' value is less than the current value, try deleting in left subtree
+    if left != null && x < value {
+      // left.delete() will return the left subtree's new root
+      var t := left.delete(x);
+      // update left subtree's root
+      left := t;
+      // remove element from ghost variable
+      elems := elems - {x};
+      // update Repr variable
+      if left != null { Repr := Repr + left.Repr; }
+    }
+
+    // if the 'x' value is higher tahn the current value, try deleting in right subtree
+    else if right != null && value < x {
+      // right.delete() will return the right subtree's new root
+      var t := right.delete(x);
+      // update right subtree's root
+      right := t;
+      // remove element from ghost variable
+      elems := elems - {x};
+      // update Repr variable
+      if right != null { Repr := Repr + right.Repr; }
+    }
+
+    // if the element that we want to delete is the current node (root),
+    // then we need to get a new root for the tree
+    else if x == value {
+      // if this node is the last one in the tree, there are no nodes left
+      if left == null && right == null {
+        node := null;
+      }
+      // if there is no left subtree, new root is the root of the right subtree
+      else if left == null {
+        node := right;
+      }
+      // if there is no right subtree, new root is the root of the left subtree
+      else if right == null {
+        node := left;
+      }
+      // if both subtrees exist, new root is the inorder successor of the node
+      else {
+        // find in order successor of the node: the leftmost (smaller) element
+        // in the right subtree
+        var min_val, new_r := right.deleteMin();
+        // update node's value
+        value := min_val;
+        // update node's right subtree root
+        right := new_r;
+        // update ghost variable
+        elems := elems - {x};
+        // update Repr variable
+        if right != null { Repr := Repr + right.Repr; }
+      }
+    }
+  }
+
+
+  // method that removes and returns the smaller element of a BST
+  // used by the delete() method when it needs to find the inorder successor
+  // of the root (i.e. the smaller element in the right subtree)
+  // returns the value of the smallest element, and the new root of the tree
+  method deleteMin() returns (min: T, node: BSTNode?)
+    decreases Repr
+    ensures fresh(Repr - old(Repr))
+    ensures node == null ==> old(elems) == {min}
+    ensures node != null ==> node.Valid() && node.Repr <= Repr && node.elems == old(elems) - {min}
+    ensures min in old(elems) && isMin(min, old(elems))
+  {
+    // the minimum element is the leftmost element in the left subtree
+    // if the current node does not have a left child, then it is the min value
+    if left == null {
+      // update values to return
+      min := value;
+      node := right;
+    }
+    // node has left child; it is not the minimum. Keep iterating through left subtree
+    else {
+      var new_lr;
+      // delete the minimum in left subtree
+      min, new_lr := left.deleteMin();
+      // update new left subtree root
+      left := new_lr;
+      // root of the tree starting at this node is still this node
+      node := this;
+      // update ghost variables
+      elems := elems - {min};
+      if left != null { Repr := Repr + left.Repr; }
+    }
+  }
+
+  // method that returns an ordered sequence of all the elements of the BST
+  // method asSeq() returns (res: seq<T>)
+  //   decreases Repr
+  //   ensures multiset(res) == multiset(elems)
+  //   ensures isSorted(res)
+  // {
+  //   // TODO: preciso de por um lemma/assert para relembrar que a BST é ordenada?
+  //   var left_seq : seq<T> := [];
+  //   var right_seq : seq<T> := [];
+  //   if left != null {
+  //     left_seq := left.asSeq();
+  //   }
+  //   if right != null {
+  //     right_seq := right.asSeq();
+  //   }
+
+  //   res := left_seq + [value] + right_seq;
+  // }
+}
+
+// **********************************************************************
+// Represents a sorted set of elements of type T. Implemented with a binary search tree
+class {:autocontracts} TreeSet {
+  // ghost variable representing a set of all the elems that are in the set
+  ghost var elems: set<T>;
+
+  // TODO: ver melhor o que é que este Repr quer dizer
+  // ghost variable representing a set of all the node objects that are in the set
+  ghost var Repr: set<object>;
+
+  // variable that represents the root of the BST that implements this sorted set
+  var root: BSTNode?
+
+  // class invariant of the TreeSet class
+  predicate Valid()
+  {
+    this in Repr &&
+    // if the root is null, then the set must be empty
+    (root == null ==> elems == {}) &&
+    // if the root exists...
+    (root != null ==> 
+      root in Repr && root.Repr <= Repr && this !in root.Repr &&
+      // check root's class invariant and connect ghost variable with its intended value
+      root.Valid() &&
+      elems == root.elems)
+  }
+
+  // constructor of the class. Creates an empty set
+  constructor()
+    ensures fresh(Repr - {this})
+    ensures elems == {}
+  {
+    root := null;
+    Repr := {this};
+    elems := {};
+  }
+
+  // method that checks if a given value is present in the set
+  // checks if it is present in the binary search tree
+  function method contains(x: T) : bool
+    ensures contains(x) <==> x in elems
+  {
+    root != null && root.contains(x)
+  }
+
+  // method that inserts a new value into the set
+  // creates a new node and inserts it in the BST
+  method insert(x: T)
+    requires x !in elems
+    ensures fresh(Repr - old(Repr))
+    ensures elems == old(elems) + {x}
+  {
+    // insert value using helper method; returns new root of BST
+    var new_root := insertAux(x, root);
+    // update BST root
+    root := new_root;
+    // update ghost variables
+    elems := root.elems;
+    Repr := root.Repr + {this};
+  }
+
+  // TODO: ver se preciso dos asserts neste method
+  // helper method for inserting a new value in the sorted set 
+  static method insertAux(x: T, n: BSTNode?) returns (new_root: BSTNode)
+    requires n == null || n.Valid()
+    modifies if n != null then n.Repr else {}
+    ensures new_root.Valid()
+    ensures n == null ==> fresh(new_root) && fresh(new_root.Repr) && new_root.elems == {x}
+    ensures n != null ==> n == new_root && fresh(n.Repr - old(n.Repr)) && n.elems == old(n.elems) + {x}
+    decreases if n == null then {} else n.Repr
+  {
+    // if the old root is empty, i.e. the set is empty
+    if n == null {
+      // just need to create a new node, that is the new root
+      new_root := new BSTNode(x);
+    }
+    // new value is equal to the current node's value; don't change anything
+    else if x == n.value {
+      new_root := n;
+    }
+    else {
+      // new value is less than current node's value; should be inserted in the left subtree
+      if x < n.value {
+        // assert n.right == null || n.right.Valid();
+        // insert in left subtree, get new root of left subtree
+        var new_lr := insertAux(x, n.left);
+        // update new root and ghost variable
+        n.left := new_lr;
+        n.Repr := n.Repr + n.left.Repr;
+      }
+      // new value is higher than current node's value; should be inserted in the right subtree
+      else {
+        // assert n.left == null || n.left.Valid();
+        // insert in right subtree, get new root of right subtree
+        var new_rr := insertAux(x, n.right);
+        // update new root and ghost variable
+        n.right := new_rr;
+        n.Repr := n.Repr + n.right.Repr;
+      }
+
+      // BST root already existed, so root didn't change 
+      new_root := n;
+      // add newly added element to the root's elems 
+      n.elems := n.elems + {x};
+    }
+  }
+
+  // method that deletes a value from the sorted set
+  method delete(x: T)
+    requires x in elems
+    ensures fresh(Repr - old(Repr))
+    ensures elems == old(elems) - {x}
+  {
+    if root != null {
+      // call delete() method from BST root, to delete the value and get new root
+      var new_root := root.delete(x);
+      // update BST root
+      root := new_root;
+      // if the new root exists, update ghost variables accordingly
+      if root != null {
+        elems := root.elems;
+        Repr := root.Repr + {this};
+      }
+      // root is null; set/BST is now empty. Reset the ghost variables
+      else {
+        elems := {};
+        Repr := {this};
+      }
+    }
+  }
+
+  // method asSeq() returns (res: seq<T>)
+  //   ensures multiset(res) == multiset(elems)
+  //   ensures isSorted(res)
+  // { 
+  //   if root != null {
+  //     res := root.asSeq();
+  //   }
+  //   else {
+  //     res := [];
+  //   }
+  // }
+  
+  // simple method that checks if the set is empty or not
+  predicate method isEmpty()
+    ensures isEmpty() <==> (|elems| == 0)
+  {
+    root == null
   }
 }
 
 // **********************************************************************
-// Represents a sorted set of elements of type T.
+// A test case, checked statically by Dafny, that covers the 
+// insert(), delete() and contains() methods of the TreeSet class
+method testTreeSetInsertionDeletion()
+{
+  // create new set
+  var s := new TreeSet();
+  // check that set is empty
+  assert s.isEmpty();
 
-// TODO: depois, ver se devia fazer com que bst fosse balanced (prob nao)
-// TODO: como ter a certeza que não há duplicados?
-class {:autocontracts} TreeSet {
-  // Ghost variable used for specification & verification purposes.
-  // Holds the set of values in the subtree starting in this node (inclusive). 
-  ghost var elems : set<T>;
+  // insert two elements
+  s.insert(2);
+  s.insert(9);
+  // check if the set is not empty anymore
+  assert !s.isEmpty();
+  // check that, for any contains() call that we do on the TreeSet,
+  // it will only be true if the argument of the call is either 2 or 9,
+  // because they are the only elements on the set
+  var x;
+  var isPresentInSet := s.contains(x);
+  assert isPresentInSet <==> x == 2 || x == 9;
+
+  // delete element
+  s.delete(9);
   
-  // Concrete state variable with internal representation (initially filled with Nil). 
-  var root: BTNode?;
+  // add new element
+  s.insert(4);
 
-  // Predicate that formalizes the class invariant. Makes sure that the binary tree starting at
-  // root is sorted (it is a binary search tree), and connects the abstract state variable (elems)
-  // to the actual set of elements in the binary tree, using the BTtoSet() function.
-  predicate Valid()
-  {
-    isBST(root) &&
-    elems == BSTtoSet(root)
-  }
+  // check that the set is not empty; still some elements left
+  assert !s.isEmpty();
+  var y;
+  var isPresentInSet2 := s.contains(y);
+  assert isPresentInSet2 <==> y == 2 || y == 4;
 
-  // Predicate that indicates if the binary tree is correctly sorted, and is a valid BST.
-  predicate isBST(node : BTNode?)
-    reads node
-    decreases root, elems
-  {
-    if node == null
-    then true
-    else (node.left != null ==> forall k :: k in BSTtoSet(node.left) ==> k < node.value) && 
-         (node.right != null ==> forall k :: k in BSTtoSet(node.right) ==> k > node.value) &&
-         isBST(node.left) && isBST(node.right)
-  }
+  // delete rest of the elements
+  s.delete(2);
+  s.delete(4);
 
-  function BSTtoSet(node : BTNode?) : set<T>
-    decreases node
-  {
-    if node == null
-    then {}
-    else {node.value} + BSTtoSet(node.left) + BSTtoSet(node.right)
-  }
+  // check that the elements that were deleted are no longer in the set
+  assert !s.contains(2);
+  assert !s.contains(4);
+  assert !s.contains(9);
 
-  // Receives the hash function to be used and initializes the set as empty.
-  constructor ()
-    ensures this.elems == {}
-  {
-    this.root := null;
-    this.elems := {};
-  }
-
-  // Inserts a new element x into the sorted set (binary search tree).
-  method insert(x : T) 
-    requires x !in elems
-    ensures elems == old(elems) + {x}
-  {
-    root := this.insertAux(x, root);
-    this.elems := this.elems + {x};
-  }
-
-  method insertAux(x : T, node : BTNode?) returns (res : BTNode?)
-  {
-    // TODO: insert method
-  }
-
-  // Deletes an element X from the sorted set (binary search tree).
-  method delete(x : T) 
-    requires x in elems
-    ensures elems == old(elems) - {x}
-  {
-    root := this.deleteAux(x, root);
-    elems := elems - {x};
-  }
-
-  method deleteAux(x : T, node : BTNode?) returns (res : BTNode?)
-  {
-    // TODO: delete method
-  }
-
-  // Check if the subtree starting in this node contains a value 'x'.
-  method contains(x: T) returns (res: bool)
-    ensures res <==> x in elems
-  {
-    res := this.containsAux(x, root);
-  }
-
-  method containsAux(x: T, node: BTNode?) returns (res: bool)
-    ensures res <==> x in BSTtoSet(node)
-  {
-    // TODO: contains method
-  }
-
-  // Returns an ordered sequence with all the elements of the BST.
-  // Need to do an inorder traversal of the tree (left subtree first, then root, then right subtree).
-  method asSeq() returns (res : seq<T>)
-    ensures multiset(res) == multiset(elems)
-    ensures forall k1, k2 :: 0 <= k1 < k2 < |res| ==> res[k1] < res[k2]
-    decreases elems
-  {
-    // TODO: talvez seja preciso lemma para provar que subtree da esquerda é menor e a da direita é maior?
-    // TODO: asSeq method
-  }
+  // check that set is empty again
+  assert s.isEmpty();
 }
 
-// -------------------------------------------
+// A test case, checked statically by Dafny, that covers the 
+// isSeq() method of the TreeSet class
+method testTreeSetSequence()
+{
+  // create new set
+  var s := new TreeSet();
+  
+  // check that the sequence that the asSeq() method returns is empty
+  // assert s.asSeq() == [];
 
-// A simple test case, checked statically by Dafny.
-method testHashSet() {
-  // TODO: fazer test case com as várias operações que a classe permite
+  // insert a bunch of elements
+  s.insert(2);
+  s.insert(3);
+  s.insert(5);
+  s.insert(4);
+  s.insert(10);
+  s.insert(1);
+  s.insert(8);
+
+  // check that the returned sequence has the same elements and is sorted
+  // assert s.asSeq() == [1, 2, 3, 4, 5, 8, 10];
+
+  // delete some of the elements
+  s.delete(1);
+  s.delete(10);
+  s.delete(3);
+  s.delete(5);
+
+  // check the sequence of elements
+  // assert s.asSeq() == [2, 4, 8];
+
+  // delete the rest of the elements
+  s.delete(2);
+  s.delete(4);
+  s.delete(8);
+
+  // check that the set is now completely empty
+  assert s.isEmpty();
+  // check that the sequence that the asSeq() method returns is now empty
+  // assert s.asSeq() == [];
+}
+
+// A test case, checked statically by Dafny, that should fail
+// because of incorrect calls to TreeSet class methods
+method testTreeSetFail()
+{
+  // create new set
+  var s := new TreeSet();
+
+  // insert some elements
+  s.insert(2);
+  s.insert(4);
+  s.insert(6);
+
+  // this method call fails the static analysis done by Dafny, because
+  // a precondition for this method is not verified: the number 7 is not
+  // on the set, so it cannot be deleted
+  s.delete(7);
+
+  // this one should also fail the static analysis, once again because it
+  // does not satisfy the precondition that an element that is already
+  // on the set cannot be inserted again
+  s.insert(2);
 }
